LeanScratch/Semantics/L1.lean
@@ -1,4 +1,6 @@
 import LeanScratch.Semantics.L1.Red
-import LeanScratch.Semantics.L1.Stx
 import LeanScratch.Semantics.L1.Step
+import LeanScratch.Semantics.L1.Stx
+import LeanScratch.Semantics.L1.Typed
+import LeanScratch.Semantics.L1.TyInfer
 
