LeanScratch/Semantics/L1/TyInfer.lean
@@ -1,0 +1,407 @@
+import LeanScratch.Semantics.L1.Stx
+import LeanScratch.Semantics.L1.Red
+import LeanScratch.Semantics.L1.Typed
+import LeanScratch.Relation
+import Batteries.Data.HashMap.Basic
+
+def Ty.infer (ctx : Ctx) : Expr → Option Ty
+  | .bool _ => some .bool
+  | .int _  => some .int
+  | .skip   => some .void
+
+  | .op a op b => do
+    let .int ← Ty.infer ctx a | none
+    let .int ← Ty.infer ctx b | none
+    match op with
+    | .add => some .int
+    | .gte => some .bool
+
+  | .deref addr => do
+    let _ ← ctx.lookup addr
+    some .int
+  | .assign addr e => do
+    let .int ← Ty.infer ctx e | none
+    let _ ← ctx.lookup addr
+    some .void
+
+  | .seq a b => do
+    let .void ← Ty.infer ctx a | none
+    Ty.infer ctx b
+
+  | .eif c a b => do
+    let .bool ← Ty.infer ctx c | none
+    let a ← Ty.infer ctx a
+    let b ← Ty.infer ctx b
+    if a = b then some a
+    else none
+
+  | .ewhile c body => do
+    let .bool ← Ty.infer ctx c    | none
+    let .void ← Ty.infer ctx body | none
+    some .void
+
+section
+
+def monize (f : α → β → γ) (h : α × β) : γ := let ⟨a, b⟩ := h; f a b
+/- def demonize () -/
+mutual
+theorem TySpec_is_infer.eqMpNone {ctx : Ctx} {e : Expr} (ih : ∀ (ty : Ty), ¬TySpec ctx e ty) : Ty.infer ctx e = none := by
+  induction e using Ty.infer.induct ctx
+  next val =>
+    exfalso
+    exact ih .bool .bool
+  next val =>
+    exfalso
+    exact ih .int .int
+  next =>
+    exfalso
+    exact ih .void .skip
+  next a op b a_ih b_ih =>
+    by_cases ha : ∃ w, TySpec ctx a w
+    · by_cases hb : ∃ w, TySpec ctx b w
+      · rcases ha with ⟨wa, pa⟩
+        rcases hb with ⟨wb, pb⟩
+
+        simp only [Ty.infer, Option.bind_eq_bind, Option.bind_eq_none]
+        intro ty ha
+        obtain rfl := TyUnique ⟨pa, TySpec_is_infer.eqMprSome ha⟩
+
+        cases wa
+        <;> simp only [Option.bind_eq_none]
+
+        intro ty hb
+        obtain rfl := TyUnique ⟨pb, TySpec_is_infer.eqMprSome hb⟩
+        cases wb
+        <;> cases op
+        <;> simp only
+        <;> exfalso
+        · exact ih .int  (.op_add pa pb)
+        · exact ih .bool (.op_gte pa pb)
+
+      · simp only [not_exists] at hb
+        simp only [Ty.infer, b_ih hb, Option.bind_eq_bind, Option.none_bind, Option.bind_eq_none]
+        intro ty _
+        cases ty
+        <;> simp only
+    · simp only [not_exists] at ha
+      simp only [Ty.infer, a_ih ha, Option.bind_eq_bind, Option.none_bind]
+  next addr =>
+    by_cases h : ∃ w, ctx.lookup addr = some w
+    · exfalso
+      exact ih .int (.deref h)
+    · simp only [← Option.ne_none_iff_exists', ne_eq, Decidable.not_not] at h
+      simp only [Ty.infer, h, Option.bind_eq_bind, Option.none_bind]
+  next addr e e_ih =>
+    by_cases h : ∃ w, TySpec ctx e w
+    · rcases h with ⟨w, p⟩
+      by_cases h : ∃ w, ctx.lookup addr = some w
+      · simp only [Ty.infer, Option.bind_eq_bind, Option.bind_eq_none]
+        intro ty h'
+        obtain rfl := TyUnique ⟨p, TySpec_is_infer.eqMprSome h'⟩
+
+        cases w
+        <;> simp only [implies_true]
+        exfalso
+        exact ih .void (.assign h p)
+
+      · simp only [← Option.ne_none_iff_exists', ne_eq, Decidable.not_not] at h
+        simp only [Ty.infer, h, Option.bind_eq_bind, Option.none_bind, Option.bind_eq_none]
+        intro ty
+        cases ty
+        <;> simp only [implies_true]
+
+    · simp only [not_exists] at h
+      simp only [Ty.infer, e_ih h, Option.bind_eq_bind, Option.none_bind]
+  next a b a_ih b_ih =>
+    by_cases ha : ∃ w, TySpec ctx a w
+    · by_cases hb : ∃ w, TySpec ctx b w
+      · simp only [Ty.infer, Option.bind_eq_bind, Option.bind_eq_none]
+        rcases ha with ⟨wa, pa⟩
+        rcases hb with ⟨wb, pb⟩
+        intro ty ha
+        obtain rfl := TyUnique ⟨pa, TySpec_is_infer.eqMprSome ha⟩
+        cases wa
+        <;> simp only
+        exfalso
+        exact ih wb (.seq pa pb)
+
+      · simp only [not_exists] at hb
+        simp only [Ty.infer, b_ih hb, Option.bind_eq_bind, Option.bind_eq_none]
+        intro ty _
+        cases ty
+        <;> simp only
+
+    · simp only [not_exists] at ha
+      simp only [Ty.infer, a_ih ha, Option.bind_eq_bind, Option.none_bind]
+  next c t f c_ih t_ih f_ih =>
+    by_cases h₁ : ∃ w, TySpec ctx c w
+    · by_cases h₂ : ∃ w, TySpec ctx t w
+      · by_cases h₃ : ∃ w, TySpec ctx f w
+        · simp only [Ty.infer, Option.bind_eq_bind, Option.bind_eq_none]
+          rcases h₁ with ⟨w₁, p₁⟩
+          rcases h₂ with ⟨w₂, p₂⟩
+          rcases h₃ with ⟨w₃, p₃⟩
+          intro ty h₁
+          obtain rfl := TyUnique ⟨p₁, TySpec_is_infer.eqMprSome h₁⟩
+          cases w₁
+          <;> simp only [Option.bind_eq_none, ite_eq_right_iff, imp_false]
+          intro ty h₂
+          obtain rfl := TyUnique ⟨p₂, TySpec_is_infer.eqMprSome h₂⟩
+          intro ty h₃
+          obtain rfl := TyUnique ⟨p₃, TySpec_is_infer.eqMprSome h₃⟩
+          by_contra!
+          rw [this] at p₂
+          exact ih w₃ (.eif p₁ p₂ p₃)
+
+        · simp only [not_exists] at h₃
+          simp only [Ty.infer, f_ih h₃, Option.bind_eq_bind, Option.none_bind, Option.bind_none,
+            Option.bind_eq_none]
+          intro ty _
+          cases ty
+          <;> simp only
+      · simp only [not_exists] at h₂
+        simp only [Ty.infer, t_ih h₂, Option.bind_eq_bind, Option.none_bind, Option.bind_eq_none]
+        intro ty _
+        cases ty
+        <;> simp only
+    · simp only [not_exists] at h₁
+      simp only [Ty.infer, c_ih h₁, Option.bind_eq_bind, Option.none_bind]
+
+  next c body c_ih body_ih =>
+    by_cases h : ∃ w, TySpec ctx c w
+    · rcases h with ⟨w, p⟩
+      by_cases h : ∃ w, TySpec ctx body w
+      · simp only [Ty.infer, Option.bind_eq_bind, Option.bind_eq_none]
+        intro ty h'
+        obtain rfl := TyUnique ⟨p, TySpec_is_infer.eqMprSome h'⟩
+        cases w
+        <;> simp only [Option.bind_eq_none]
+        rcases h with ⟨w', p'⟩
+        intro ty h'
+        obtain rfl := TyUnique ⟨p', TySpec_is_infer.eqMprSome h'⟩
+        cases w'
+        <;> simp only
+
+        exact ih .void (.ewhile p p')
+      · simp only [not_exists] at h
+        simp only [Ty.infer, body_ih h, Option.bind_eq_bind, Option.none_bind, Option.bind_eq_none]
+        intro ty _
+        cases ty
+        <;> simp only
+
+    · simp only [not_exists] at h
+      simp only [Ty.infer, c_ih h, Option.bind_eq_bind, Option.none_bind]
+
+theorem TySpec_is_infer.eqMprNone {ctx : Ctx} {e : Expr} (ih : Ty.infer ctx e = none) (ty : Ty) : ¬TySpec ctx e ty := by
+  intro cont
+  induction e generalizing ty
+  <;> try { simp only [Ty.infer] at ih; done }
+  <;> cases cont
+
+  case op tya tyb =>
+    simp only [Ty.infer, TySpec_is_infer.eqMpSome tya, TySpec_is_infer.eqMpSome tyb,
+      Option.bind_eq_bind, Option.some_bind] at ih
+
+  case op_gte tya tyb =>
+    simp only [Ty.infer, TySpec_is_infer.eqMpSome tya, TySpec_is_infer.eqMpSome tyb,
+      Option.bind_eq_bind, Option.some_bind] at ih
+
+  case eif c t f =>
+    simp only [Ty.infer, TySpec_is_infer.eqMpSome c, TySpec_is_infer.eqMpSome t,
+      TySpec_is_infer.eqMpSome f, Option.bind_eq_bind, Option.some_bind, ↓reduceIte] at ih
+
+  case ewhile c body =>
+    simp only [Ty.infer, TySpec_is_infer.eqMpSome c, TySpec_is_infer.eqMpSome body,
+      Option.bind_eq_bind, Option.some_bind] at ih
+  case assign e _ h_addr ty =>
+    rcases h_addr with ⟨w', p'⟩
+    simp only [Ty.infer, TySpec_is_infer.eqMpSome ty, p', Option.bind_eq_bind, Option.some_bind]
+      at ih
+
+  case deref addr =>
+    rcases addr with ⟨_, p⟩
+    simp only [Ty.infer, p, Option.bind_eq_bind, Option.some_bind] at ih
+  case seq tya tyb=>
+    simp only [
+      Ty.infer,
+      TySpec_is_infer.eqMpSome tya,
+      TySpec_is_infer.eqMpSome tyb,
+      Option.bind_eq_bind,
+      Option.some_bind
+    ] at ih
+
+theorem TySpec_is_infer.eqMpSome {ctx : Ctx} {e : Expr} {ty : Ty} (ih : TySpec ctx e ty) : Ty.infer ctx e = some ty := by
+  induction ih
+  <;> simp only [Ty.infer, Option.bind_eq_bind]
+  <;> try simp_all only [Option.some_bind, ite_true]
+  case deref h =>
+    rcases h with ⟨_, p⟩
+    simp only [p, Option.some_bind]
+  case assign h _ _ =>
+    rcases h with ⟨_, p⟩
+    simp only [p, Option.some_bind]
+
+theorem TySpec_is_infer.eqMprSome {ctx : Ctx} {e : Expr} {ty : Ty} (ih : Ty.infer ctx e = some ty) : TySpec ctx e ty := by
+  induction e generalizing ty
+  <;> simp only [Ty.infer, Option.bind_eq_bind, Option.some.injEq] at ih
+  case bool =>
+    rw [← ih]
+    exact .bool
+  case int =>
+    rw [← ih]
+    exact .int
+  case skip =>
+    rw [← ih]
+    exact .skip
+  case op lhs op rhs lhs_ih rhs_ih =>
+    by_cases h : ∃ ty, Ty.infer ctx lhs = some ty
+    <;> by_cases h' : ∃ ty, Ty.infer ctx rhs = some ty
+    · rcases h  with ⟨w₁, p₁⟩
+      rcases h' with ⟨w₂, p₂⟩
+      cases w₁
+      <;> cases w₂
+      <;> simp only [p₁, p₂, Option.some_bind] at ih
+      cases op
+      <;> simp only [Option.some.injEq] at ih
+      <;> rw [←ih]
+      · exact .op_add (lhs_ih p₁) (rhs_ih p₂)
+      · exact .op_gte (lhs_ih p₁) (rhs_ih p₂)
+    · rcases h with ⟨w, h⟩
+      simp only [← Option.ne_none_iff_exists', ne_eq, not_not] at h'
+      cases w
+      <;> simp only [h, h', Option.none_bind, Option.some_bind] at ih
+    · rcases h' with ⟨w, h'⟩
+      simp only [← Option.ne_none_iff_exists', ne_eq, not_not] at h
+      cases w
+      <;> simp only [h, h', Option.none_bind, Option.some_bind] at ih
+    · simp only [← Option.ne_none_iff_exists', ne_eq, not_not] at *
+      simp only [h, h', Option.none_bind, Option.some_bind] at ih
+
+  case eif cond t f cond_ih t_ih f_ih =>
+    by_cases h : ∃ ty, Ty.infer ctx cond = some ty
+    case neg =>
+      simp only [← Option.ne_none_iff_exists', ne_eq, not_not] at h
+      simp only [h, Option.none_bind, Option.some_bind] at ih
+
+    rcases h with ⟨w, p⟩
+    rw [p] at ih
+    cases w
+    <;> simp only [Option.some_bind] at ih
+
+    by_cases h : ∃ ty, Ty.infer ctx t = some ty
+    <;> by_cases h' : ∃ ty, Ty.infer ctx f = some ty
+    · rcases h  with ⟨w₁, p₁⟩
+      rcases h' with ⟨w₂, p₂⟩
+      simp only [p₁, p₂, Option.some_bind, ite_some_none_eq_some] at ih
+      rcases ih with ⟨w_eq, out⟩
+      have : w₁ = w₂ := by cases w₁ <;> cases w₂ <;> trivial
+      simp only [this] at *
+      rw [← out]
+      exact .eif (cond_ih p) (t_ih p₁) (f_ih p₂)
+
+    · rcases h with ⟨w, h⟩
+      simp only [← Option.ne_none_iff_exists', ne_eq, not_not] at h'
+      cases w
+      <;> simp only [h, h', Option.none_bind, Option.some_bind] at ih
+
+    · rcases h' with ⟨w, h'⟩
+      simp only [← Option.ne_none_iff_exists', ne_eq, not_not] at h
+      cases w
+      <;> simp only [h, h', Option.none_bind, Option.some_bind] at ih
+    · simp only [← Option.ne_none_iff_exists', ne_eq, not_not] at *
+      simp only [h, h', Option.none_bind, Option.some_bind] at ih
+
+  case ewhile cond e cond_ih e_ih => 
+    by_cases h : ∃ ty, Ty.infer ctx cond = some ty
+    <;> by_cases h' : ∃ ty, Ty.infer ctx e = some ty
+    · rcases h  with ⟨w₁, p₁⟩
+      rcases h' with ⟨w₂, p₂⟩
+      cases w₁
+      <;> cases w₂
+      <;> simp only [p₁, p₂, Option.some_bind, Option.some.injEq] at ih
+      rw [← ih]
+      exact .ewhile (cond_ih p₁) (e_ih p₂)
+    · rcases h with ⟨w, h⟩
+      simp only [← Option.ne_none_iff_exists', ne_eq, not_not] at h'
+      cases w
+      <;> simp only [h, h', Option.none_bind, Option.some_bind] at ih
+    · rcases h' with ⟨w, h'⟩
+      simp only [← Option.ne_none_iff_exists', ne_eq, not_not] at h
+      cases w
+      <;> simp only [h, h', Option.none_bind, Option.some_bind] at ih
+    · simp only [← Option.ne_none_iff_exists', ne_eq, not_not] at *
+      simp only [h, h', Option.none_bind, Option.some_bind] at ih
+
+  case assign addr e e_ih =>
+    by_cases h : ∃ ty, Ty.infer ctx e = some ty
+    · rcases h with ⟨w, p⟩
+      rw [p] at ih
+      cases w
+      <;> simp only [Option.some_bind] at ih
+      by_cases h' : ∃ w, ctx.lookup addr = some w
+      · rcases h' with ⟨w, h'⟩
+        simp only [h', Option.some_bind, Option.some.injEq] at ih
+        rw [← ih]
+        exact .assign (Exists.intro w h') (e_ih p)
+
+      · simp only [← Option.ne_none_iff_exists', ne_eq, Decidable.not_not] at h'
+        simp only [h', Option.none_bind] at ih
+
+    · simp only [← Option.ne_none_iff_exists', ne_eq, not_not] at h
+      simp only [h, Option.none_bind, Option.some_bind] at ih
+  case deref addr =>
+    by_cases h : ∃ w, ctx.lookup addr = some w
+    · rcases h with ⟨w, h⟩
+      simp only [h, Option.some_bind, Option.some.injEq] at ih
+      rw [← ih]
+      exact .deref (Exists.intro w h)
+
+    · simp only [← Option.ne_none_iff_exists', ne_eq, Decidable.not_not] at h
+      simp only [h, Option.none_bind] at ih
+
+  case seq a b a_ih b_ih =>
+    by_cases h : ∃ ty, Ty.infer ctx a = some ty
+    <;> by_cases h' : ∃ ty, Ty.infer ctx b = some ty
+    · rcases h  with ⟨w₁, p₁⟩
+      rcases h' with ⟨w₂, p₂⟩
+      cases w₁
+      <;> simp only [p₁, p₂, Option.some_bind, Option.some.injEq] at ih
+      rw [← ih]
+      exact .seq (a_ih p₁) (b_ih p₂)
+
+    · rcases h with ⟨w, h⟩
+      simp only [← Option.ne_none_iff_exists', ne_eq, not_not] at h'
+      cases w
+      <;> simp only [h, h', Option.none_bind, Option.some_bind] at ih
+
+    · rcases h' with ⟨w, h'⟩
+      simp only [← Option.ne_none_iff_exists', ne_eq, not_not] at h
+      cases w
+      <;> simp only [h, h', Option.none_bind, Option.some_bind] at ih
+
+    · simp only [← Option.ne_none_iff_exists', ne_eq, not_not] at *
+      simp only [h, h', Option.none_bind, Option.some_bind] at ih
+end
+
+theorem TySpec_is_infer : Relation.optRel (monize TySpec) = Relation.graph (monize Ty.infer) := by
+  apply funext₂
+  intro ⟨ctx, e⟩ post
+  apply propext
+
+  constructor
+  <;> intro ih
+  <;> cases post
+  <;> simp only [Relation.graph, Prod.exists, not_exists, Relation.optRel, monize] at *
+
+  case mp.none =>
+    exact TySpec_is_infer.eqMpNone ih
+  case mpr.none =>
+    exact TySpec_is_infer.eqMprNone ih
+  case mp.some ty =>
+    exact TySpec_is_infer.eqMpSome ih
+  case mpr.some ty =>
+    exact TySpec_is_infer.eqMprSome ih
+
+/-- info: 'TySpec_is_infer' depends on axioms: [Quot.sound, propext, Classical.choice] -/
+#guard_msgs in #print axioms TySpec_is_infer
+end
