LeanScratch/Semantics/L1/Typed.lean
@@ -1,0 +1,247 @@
+import LeanScratch.Semantics.L1.Stx
+import LeanScratch.Semantics.L1.Red
+import LeanScratch.Relation
+import Mathlib.Data.List.AList
+
+inductive Ty
+  | bool
+  | int
+  | void
+deriving DecidableEq
+
+-- TODO: Change Int to Unit
+abbrev Ctx := AList fun _ : String => Int
+
+inductive TySpec : Ctx → Expr → Ty → Prop
+  | bool : TySpec _ (.bool b) .bool
+  | int  : TySpec _ (.int i)  .int
+  | skip : TySpec _ .skip     .void
+
+  | op_add : TySpec ctx a .int → TySpec ctx b .int
+      → TySpec ctx (.op a .add b) .int
+  | op_gte : TySpec ctx a .int → TySpec ctx b .int
+      → TySpec ctx (.op a .gte b) .bool
+
+  | deref : (h : ∃ w, ctx.lookup addr = some w) 
+      → TySpec ctx (.deref addr) .int
+  | assign : (h : ∃ w, ctx.lookup addr = some w) → TySpec ctx e .int
+      → TySpec ctx (.assign addr e) .void
+  | seq : TySpec ctx a .void → TySpec ctx b o
+      → TySpec ctx (.seq a b) o
+
+  | eif : TySpec ctx c .bool → TySpec ctx t a → TySpec ctx f a
+      → TySpec ctx (.eif c t f) a
+
+  | ewhile : TySpec ctx c .bool → TySpec ctx body .void
+      → TySpec ctx (.ewhile c body) .void
+
+theorem TyUnique : TySpec ctx i o₁ ∧ TySpec ctx i o₂ → o₁ = o₂ := by
+  rintro ⟨a, b⟩
+
+  induction a generalizing o₂
+  <;> cases b
+  <;> try rfl
+  case seq b_ih _ ba =>
+    exact b_ih ba
+  case eif t_ih _ _ ta _ =>
+    exact t_ih ta
+
+theorem AddrConsistency (trans : Red w₁ w₂) : (∃ w, w₁.snd.lookup addr = some w) → ∃ w, w₂.snd.lookup addr = some w := by
+  intro h
+  induction trans
+  <;> simp_all only
+  next addr' v _ _ =>
+  by_cases h₂ : addr = addr'
+  · use v
+    simp [←h₂]
+  · simp [←ne_eq] at h₂
+    rcases h with ⟨w, p⟩
+    use w
+    simp only [AList.lookup_insert_ne h₂]
+    exact p
+
+theorem CtxConsistency (trans : Red ⟨e, s⟩ ⟨e', s'⟩) (a : TySpec s w x) : TySpec s' w x := by
+  induction a
+  · exact .bool
+  · exact .int
+  · exact .skip
+  case op_add a b => exact .op_add a b
+  case op_gte a b => exact .op_gte a b
+  case deref h =>
+    exact .deref (AddrConsistency trans h)
+  case assign h _ deeper =>
+    exact .assign (AddrConsistency trans h) deeper
+  case seq a b => exact .seq a b
+  case eif c t f => exact .eif c t f
+  case ewhile c b => exact .ewhile c b
+
+
+theorem TypePreservation : Red ⟨e, s⟩ ⟨e', s'⟩ → TySpec s e x → TySpec s' e' x := by
+  intro h spec
+  induction spec generalizing e' s'
+  <;> cases h
+  <;> try trivial
+  · exact .int
+  case op_add.op1 rhs lhs_ih _ _ a =>
+    exact .op_add (lhs_ih a) (CtxConsistency a rhs)
+  case op_add.op2 lhs _ _ rhs_ih _ _ a =>
+    exact .op_add (CtxConsistency a lhs) (rhs_ih a)
+  · exact .bool
+  case op_gte.op1 rhs lhs_ih _ _ a =>
+    exact .op_gte (lhs_ih a) (CtxConsistency a rhs)
+  case op_gte.op2 lhs _ _ rhs_ih _ _ a =>
+    exact .op_gte (CtxConsistency a lhs) (rhs_ih a)
+  · exact .int
+  · exact .skip
+  case assign2 h _ a_ih _ a =>
+    exact .assign (AddrConsistency a h) (a_ih a)
+  case seq2 o a_ih _ _ a =>
+    exact .seq (a_ih a) (CtxConsistency a o)
+  case eif.if_cond t f c_ih _ _ _ a =>
+    exact .eif (c_ih a) (CtxConsistency a t) (CtxConsistency a f)
+  case ewhile c b _ _ =>
+    exact .eif c (.seq b (.ewhile c b)) .skip
+
+/-- info: 'TypePreservation' depends on axioms: [propext, Quot.sound] -/
+#guard_msgs in #print axioms TypePreservation
+
+theorem Progress (spec : TySpec s e x) : (e.isValue ∨ ∃ w, Red ⟨e, s⟩ w) := by
+  induction spec
+  · left; simp only [Expr.isValue]
+  · left; simp only [Expr.isValue]
+  · left; simp only [Expr.isValue]
+  case op_add a b ta tb a_ih b_ih =>
+    right
+    cases a_ih
+    case inl h =>
+      cases a
+      <;> simp only [Expr.isValue] at h
+      <;> cases ta
+      next a =>
+      cases b_ih
+      case inl h =>
+        cases b
+        <;> simp only [Expr.isValue] at h
+        <;> cases tb
+        next b =>
+        use ⟨.int (a + b), s⟩
+        exact .op_add a b
+
+      case inr h =>
+        rcases h with ⟨⟨e', s'⟩, p⟩
+        use ⟨.op (.int a) .add e', s'⟩
+        exact .op2 p (by simp only [Expr.isInt])
+
+    case inr h =>
+      rcases h with ⟨⟨e', s'⟩, p⟩
+      use ⟨e'.op .add b, s'⟩
+      exact .op1 p
+  case op_gte a b ta tb a_ih b_ih =>
+    right
+    cases a_ih
+    case inl h =>
+      cases a
+      <;> simp only [Expr.isValue] at h
+      <;> cases ta
+      next a =>
+      cases b_ih
+      case inl h =>
+        cases b
+        <;> simp only [Expr.isValue] at h
+        <;> cases tb
+        next b =>
+        use ⟨.bool (a ≥ b), s⟩
+        exact .op_gte a b
+
+      case inr h =>
+        rcases h with ⟨⟨e', s'⟩, p⟩
+        use ⟨.op (.int a) .gte e', s'⟩
+        exact .op2 p (by simp only [Expr.isInt])
+
+    case inr h =>
+      rcases h with ⟨⟨e', s'⟩, p⟩
+      use ⟨.op e' .gte b, s'⟩
+      exact .op1 p
+
+  case deref addr h =>
+    right
+    rcases h with ⟨w, p⟩
+    use ⟨.int w, s⟩
+    exact .deref p
+  case assign e addr h ba_ih x =>
+    right
+    cases x
+    case inl h =>
+      cases e
+      <;> simp only [Expr.isValue] at h
+      <;> cases ba_ih
+      next h' val =>
+      use ⟨.skip, s.insert addr val⟩
+      exact .assign1 h'
+    case inr h =>
+      rcases h with ⟨⟨e', s'⟩, p⟩
+      use ⟨.assign addr e', s'⟩
+      exact .assign2 p
+
+  case seq ea eb _ a _ a_ih _ =>
+    right
+    cases a_ih
+    case inl h =>
+      use ⟨eb, s⟩
+      rcases ea
+      <;> simp only [Expr.isValue] at h
+      <;> cases a
+      exact .seq1
+
+    case inr h =>
+      rcases h with ⟨⟨e', s'⟩, p⟩
+      use ⟨.seq e' eb, s'⟩
+      exact .seq2 p
+  case eif ec et _ ef c _ _ c_ih _ _ =>
+    right
+    cases c_ih
+    case inl h =>
+      cases ec
+      <;> simp only [Expr.isValue] at h
+      <;> cases c
+      next val =>
+      cases val
+      · use ⟨ef, s⟩
+        exact .if_f
+      · use ⟨et, s⟩
+        exact .if_t
+    case inr h =>
+      rcases h with ⟨⟨e', s'⟩ , p⟩
+      use ⟨.eif e' et ef, s'⟩
+      exact .if_cond p
+
+  case ewhile c body _ _ _ _ =>
+    right
+    use ⟨.eif c (.seq body (.ewhile c body)) .skip, s⟩
+    exact .ewhile
+
+/-- info: 'Progress' depends on axioms: [propext, Quot.sound] -/
+#guard_msgs in #print axioms Progress
+
+theorem LongTypePreservation (spec : TySpec s e ty) (h : RedStar ⟨e, s⟩ ⟨e', s'⟩) : TySpec s' e' ty := by
+  have (w₁ w₂) (spec : TySpec w₁.snd w₁.fst ty) (h : RedStar w₁ w₂) : TySpec w₂.snd w₂.fst ty := by
+    induction h
+    case base base =>
+      exact TypePreservation base spec
+    case rfl => exact spec
+    case trans l1_ih l2_ih =>
+      exact l2_ih $ l1_ih spec
+  have := this ⟨e, s⟩ ⟨e', s'⟩
+  simp only at this
+  exact this spec h
+
+theorem Safety (spec : TySpec s e ty) (h : RedStar ⟨e, s⟩ ⟨e', s'⟩) : (e'.isValue ∨ ∃ w₃, Red ⟨e', s'⟩ w₃) := by
+  cases h
+  case base base =>
+    exact Progress (TypePreservation base spec)
+  case rfl => exact Progress spec
+  case trans l1 l2 =>
+    exact Progress $ (LongTypePreservation · l2) ∘ (LongTypePreservation · l1) $ spec
+
+/-- info: 'Safety' depends on axioms: [propext, Quot.sound] -/
+#guard_msgs in #print axioms Safety
